P1  M1 P2    <-  P3  a
P4  M2 P5    <-  P6  b
P7  M3 P8    <-  P9  c
P10 M4 P11   <-  P12 x0


eixox'
x=cos(deg((x(P9)-x(M3))))*x
y=sin(deg((x(P9)-x(M3))))*x

eixoy'
x=-sin(deg((x(P9)-x(M3))))*y
y=cos(deg((x(P9)-x(M3))))*y


eixox''
x=cos(deg(x(P9)-x(M3)))*x-sin(deg(x(P9)-x(M3)))*(x(P21)-x(M5))
y=sin(deg(x(P9)-x(M3)))*x+cos(deg(x(P9)-x(M3)))*(x(P21)-x(M5))


eixoy''
x=cos(deg(x(P9)-x(M3)))*(x(P12)-x(M4))-sin(deg(x(P9)-x(M3)))*y
y=sin(deg(x(P9)-x(M3)))*(x(P12)-x(M4))+cos(deg(x(P9)-x(M3)))*y


assintota1
x=cos(deg(x(P9)-x(M3)))*((x(P12)-x(M4))+(x(P3)-x(P1))*t)-sin(deg(x(P9)-x(M3)))*((x(P21)-x(M5))+(x(P6)-x(P4))*t)
y=sin(deg(x(P9)-x(M3)))*((x(P12)-x(M4))+(x(P3)-x(P1))*t)+cos(deg(x(P9)-x(M3)))*((x(P21)-x(M5))+(x(P6)-x(M2))*t)


assintota2
x=cos(deg(x(P9)-x(M3)))*((x(P12)-x(M4))-(x(P3)-x(P1))*t)-sin(deg(x(P9)-x(M3)))*((x(P21)-x(M5))+(x(P6)-x(P4))*t)
y=sin(deg(x(P9)-x(M3)))*((x(P12)-x(M4))-(x(P3)-x(P1))*t)+cos(deg(x(P9)-x(M3)))*((x(P21)-x(M5))+(x(P6)-x(P4))*t)


hiperboley1
x=cos(deg(x(P9)-x(M3)))*((x(P12)-x(M4))+(x(P3)-x(P1))*(exp(t)-exp(-t))/2)-sin(deg(x(P9)-x(M3)))*((x(P21)-x(M5))+(x(P6)-x(P4))*(exp(t)+exp(-t))/2)
y=sin(deg(x(P9)-x(M3)))*((x(P12)-x(M4))+(x(P3)-x(P1))*(exp(t)-exp(-t))/2)+cos(deg(x(P9)-x(M3)))*((x(P21)-x(M5))+(x(P6)-x(P4))*(exp(t)+exp(-t))/2)

hiperboley2
x=cos(deg(x(P9)-x(M3)))*((x(P12)-x(M4))+(x(P3)-x(P1))*(exp(t)-exp(-t))/2)-sin(deg(x(P9)-x(M3)))*((x(P21)-x(M5))-(x(P6)-x(P4))*(exp(t)+exp(-t))/2)
y=sin(deg(x(P9)-x(M3)))*((x(P12)-x(M4))+(x(P3)-x(P1))*(exp(t)-exp(-t))/2)+cos(deg(x(P9)-x(M3)))*((x(P21)-x(M5))-(x(P6)-x(P4))*(exp(t)+exp(-t))/2)

t=-2:2