

assintota1
x=(cos(tht)*a-sin(tht)*b)*exp(2)/2
y=(sin(tht)*a+cos(tht)*b)*exp(2)/2


x=cos(tht)*(x0+a*exp(2)/2)-sin(tht)*(y0+b*exp(2)/2)
y=sin(tht)*(x0+a*exp(2)/2)+cos(tht)*(y0+b*exp(2)/2)


assintota2
x=(-cos(tht)*a-sin(tht)*b)*exp(2)/2
y=(-sin(tht)*a+cos(tht)*b)*exp(2)/2

x=cos(tht)*(x0-a*exp(2)/2)-sin(tht)*(y0+b*exp(2)/2)
y=sin(tht)*(x0-a*exp(2)/2)+cos(tht)*(y0+b*exp(2)/2)


hiperbolex1
x=cos(tht)*(a*(exp(t)+exp(-t))/2)-sin(tht)*(b*(exp(t)-exp(-t))/2)
y=sin(tht)*(a*(exp(t)+exp(-t))/2)+cos(tht)*(b*(exp(t)-exp(-t))/2)


x=cos(tht)*(x0+a*(exp(t)+exp(-t))/2)-sin(tht)*(y0+b*(exp(t)-exp(-t))/2)
y=sin(tht)*(x0+a*(exp(t)+exp(-t))/2)+cos(tht)*(y0+b*(exp(t)-exp(-t))/2)


hiperbolex2
x=cos(tht)*(-a*(exp(t)+exp(-t))/2)-sin(tht)*(-b*(exp(t)-exp(-t))/2)
y=sin(tht)*(-a*(exp(t)+exp(-t))/2)+cos(tht)*(-b*(exp(t)-exp(-t))/2)


x=cos(tht)*(x0-a*(exp(t)+exp(-t))/2)-sin(tht)*(y0-b*(exp(t)-exp(-t))/2)
y=sin(tht)*(x0-a*(exp(t)+exp(-t))/2)+cos(tht)*(y0-b*(exp(t)-exp(-t))/2)


t=-2:2

eixox'
x1
x=a*(exp(2)+exp(-2))/2*x(V)/sqrt(x(V)^2+y(V)^2)
y=a*(exp(2)+exp(-2))/2*y(V)/sqrt(x(V)^2+y(V)^2)

x=if((a*exp(2)/2+x0)>1,(a*exp(2)/2+x0)*x(V)/sqrt(x(V)^2+y(V)^2),x(V)/sqrt(x(V)^2+y(V)^2))
y=if((a*exp(2)/2+x0)>1,(a*exp(2)/2+x0)*y(V)/sqrt(x(V)^2+y(V)^2),y(V)/sqrt(x(V)^2+y(V)^2))

x1n
x=-a*(exp(2)+exp(-2))/2*x(V)/sqrt(x(V)^2+y(V)^2)
y=-a*(exp(2)+exp(-2))/2*y(V)/sqrt(x(V)^2+y(V)^2)

eixoy'
y1
x=b*(exp(2)-exp(-2))/2*cos(tht+90)
y=b*(exp(2)-exp(-2))/2*sin(tht+90)

x=if((b*exp(2)/2+y0)>1,(b*exp(2)/2+y0)*cos(tht+90),cos(tht+90))
y=if((b*exp(2)/2+y0)>1,(b*exp(2)/2+y0)*sin(tht+90),sin(tht+90))

y1n
x=-b*(exp(2)-exp(-2))/2*cos(tht+90)
y=-b*(exp(2)-exp(-2))/2*sin(tht+90)

x=if((-b*exp(2)/2+y0)<0,(-b*exp(2)/2+y0)*cos(tht+90),0)
y=if((-b*exp(2)/2+y0)<0,(-b*exp(2)/2+y0)*sin(tht+90),0)


eixo x''
x2
x=if(x0+a*exp(2)/2>1,cos(tht)*(x0+a*exp(2)/2)-sin(tht)*y0,cos(tht)-sin(tht)*y0)
y=if(x0+a*exp(2)/2>1,sin(tht)*(x0+a*exp(2)/2)+cos(tht)*y0,sin(tht)+cos(tht)*y0)

x2n
x=if(x0-a*exp(2)/2<0,cos(tht)*(x0-a*exp(2)/2)-sin(tht)*y0,-sin(tht)*y0)
y=if(x0-a*exp(2)/2<0,sin(tht)*(x0-a*exp(2)/2)+cos(tht)*y0,cos(tht)*y0)

eixo y''
y2
x=if((b*exp(2)/2+y0)>1,cos(tht)*x0-(b*exp(2)/2+y0)*sin(tht),cos(tht)*x0-sin(tht))
y=if((b*exp(2)/2+y0)>1,sin(tht)*x0+(b*exp(2)/2+y0)*cos(tht),sin(tht)*x0+cos(tht))

y2n
x=if((-b*exp(2)/2+y0)<0,cos(tht)*x0-(-b*exp(2)/2+y0)*sin(tht),cos(tht)*x0)
y=if((-b*exp(2)/2+y0)<0,sin(tht)*x0+(-b*exp(2)/2+y0)*cos(tht),sin(tht)*x0)


eixo x
x=abs(cos(tht))*(abs(x0)+a*exp(2)/2)+abs(sin(tht))*(abs(y0)+b*exp(2)/2)

eixo y
y=abs(sin(tht))*(abs(x0)+a*exp(2)/2)+abs(cos(tht))*(abs(y0)+b*exp(2)/2)
